Updated examples to work with changes to communication layer

src/request_response/DY.Example.RequestResponse.Protocol.Stateful.Proof.fst
@@ -19,16 +19,16 @@ let state_predicates_protocol: local_state_predicate protocol_state = {
     | ClientSendRequest {server; cmeta_data; nonce} -> (
       let client = prin in
       comm_meta_data_knowable tr client cmeta_data /\
-      is_secret (join (principal_label client) (principal_label server)) tr nonce
+      is_secret (comm_label client server) tr nonce
     )
     | ServerReceiveRequest {client; nonce} -> (
       let server = prin in
-      is_knowable_by (join (principal_label client) (principal_label server)) tr nonce
+      is_knowable_by (comm_label client server) tr nonce
     )
     | ClientReceiveResponse {server; cmeta_data; nonce} -> (
       let client = prin in
       comm_meta_data_knowable tr client cmeta_data /\
-      is_secret (join (principal_label client) (principal_label server)) tr nonce
+      is_secret (comm_label client server) tr nonce
     )
   );
   pred_later = (fun tr1 tr2 prin sess_id state -> ());
@@ -55,7 +55,7 @@ let comm_layer_event_preds = {
   send_request = (fun tr client server (payload:message_t) key_label ->
     match payload with
     | Request {client; nonce} -> (
-      is_secret (join (principal_label client) (principal_label server)) tr nonce
+      is_secret (comm_label client server) tr nonce
     )
     | Response {b} -> True
   );
@@ -138,7 +138,7 @@ let client_send_request_proof tr comm_keys_ids client server =
   ()
 #pop-options
 
-#push-options "--ifuel 1 --z3rlimit 80"
+#push-options "--ifuel 1 --z3rlimit 85"
 val server_receive_request_send_response_proof:
   tr:trace ->
   comm_keys_ids:communication_keys_sess_ids ->
@@ -155,12 +155,28 @@ val server_receive_request_send_response_proof:
   [SMTPat (trace_invariant tr); SMTPat (server_receive_request_send_response comm_keys_ids server msg_id tr)]
 let server_receive_request_send_response_proof tr comm_keys_ids server msg_id =
   assert(apply_com_layer_lemmas comm_layer_event_preds);
+  let (_, tr_out) = server_receive_request_send_response comm_keys_ids server msg_id tr in
   match receive_request comm_keys_ids server msg_id tr with
-  | (None, tr) -> ()
-  | (Some (msg, cmeta_data), tr) -> (
-    assert(is_well_formed message_t (is_knowable_by (get_response_label tr cmeta_data) tr) msg);
+  | (None, tr) -> assert(tr == tr_out)
+  | (Some (Request req, cmeta_data), tr) -> (
+    let send_event client = CommClientSendRequest client server (serialize message_t (Request req)) cmeta_data.key in
+    assert(trace_invariant tr);
+    eliminate (exists client. event_triggered tr client (send_event client)) \/
+              is_publishable tr cmeta_data.key
+    returns is_knowable_by (comm_label req.client server) tr req.nonce
+    with _. eliminate exists client. event_triggered tr client (send_event client)
+      returns _
+      with _. (
+        let i = find_event_triggered_at_timestamp tr client (send_event client) in
+        // Triggers event_triggered_at_implies_pred
+        assert(event_triggered_at tr i client (send_event client));
+        // From protocol event predicate
+        assert(is_knowable_by (comm_label req.client server) tr req.nonce)
+      )
+    and _. assert(is_well_formed message_t (is_publishable tr) (Request req));
     ()
   )
+  | (Some _, tr) -> assert(tr == tr_out)
 #pop-options
 
 #push-options "--ifuel 4 --z3rlimit 40"
